test/Test/Parse.lean
@@ -1,14 +1,15 @@
 import Time
 
 open Time
+open Time.Notation
+
 open Lean Parsec
 
 -- Date
 
 def parseDate? (fmt : String) (s : String) : Option Date := parse TimeLocale.deDETimeLocale fmt s
 
-def dtDate : Date := { Year := 2023, Month := ⟨2, (by simp_arith)⟩,
-                       Day := ⟨12, (by simp_arith)⟩, IsValid := (by simp_arith) }
+def dtDate : Date := date% 2023-2-12
 
 example : (toGregorian <| fromGregorianDate dtDate) == dtDate := by rfl
 
@@ -31,30 +32,34 @@ example : parseDate? "%Y-%V-%A" "2023-06-Sonntag" == some dtDate := by native_de
 def parseTimeOfDay? (fmt : String) (s : String) : Option TimeOfDay :=
   parse TimeLocale.defaultTimeLocale fmt s
 
-def dtTimeOfDay (nanoSecs : Nat) : Option TimeOfDay :=
-    some { Hour := ⟨12, (by simp_arith)⟩, Minute := ⟨24, (by simp_arith)⟩,
-           Second := TimeOfDay.toSecond 30 nanoSecs (by simp_arith) (by simp_arith)}
+def dtTimeOfDay1 : TimeOfDay := time% 12:24:30
 
-example : parseTimeOfDay? "%H:%M:%S" "12:24:30" == dtTimeOfDay 0 := by native_decide
+def dtTimeOfDay2 : TimeOfDay := time% 12:24:30.1234
 
-example : parseTimeOfDay? "%H:%M:%S%Q" "12:24:30.1234" == dtTimeOfDay 123400000 := by native_decide
+def dtTimeOfDay3 : TimeOfDay := time% 12:24:30.000000020
 
-example : parseTimeOfDay? "%H:%M:%S%Q" "12:24:30" == dtTimeOfDay 0 := by native_decide
+example : dtTimeOfDay2.Second.val.val = 30123400000 := by rfl
 
-example : parseTimeOfDay? "%H:%M:%S.%q" "12:24:30.000000020" == dtTimeOfDay 20 := by native_decide
+example : dtTimeOfDay3.Second.val.val = 30000000020 := by rfl
 
-example : parseTimeOfDay? "%R:%S" "12:24:30" == dtTimeOfDay 0 := by native_decide
+example : parseTimeOfDay? "%H:%M:%S" "12:24:30" == dtTimeOfDay1 := by native_decide
 
-example : parseTimeOfDay? "%T" "12:24:30" == dtTimeOfDay 0 := by native_decide
+example : parseTimeOfDay? "%H:%M:%S%Q" "12:24:30.1234" == dtTimeOfDay2 := by native_decide
+
+example : parseTimeOfDay? "%H:%M:%S%Q" "12:24:30" == dtTimeOfDay1 := by native_decide
+
+example : parseTimeOfDay? "%H:%M:%S.%q" "12:24:30.000000020" == dtTimeOfDay3 := by native_decide
+
+example : parseTimeOfDay? "%R:%S" "12:24:30" == dtTimeOfDay1 := by native_decide
+
+example : parseTimeOfDay? "%T" "12:24:30" == dtTimeOfDay1 := by native_decide
 
 -- LocalTime
 
 def parseLocalTime? (fmt : String) (s : String) : Option LocalTime :=
   parse TimeLocale.defaultTimeLocale fmt s
 
-def dtLocalTime : Option LocalTime :=
-  some ⟨fromGregorianDate dtDate,
-    ⟨12, (by simp_arith)⟩, ⟨24, (by simp_arith)⟩, TimeOfDay.toSecond 30 0 (by simp_arith) (by simp_arith)⟩
+def dtLocalTime : LocalTime := datetime% 2023-2-12 12:24:30
 
 example : parseLocalTime? "%Y%m%d%H%M%S" "20230212122430" == dtLocalTime := by native_decide
 
@@ -66,9 +71,7 @@ example : parseLocalTime? "%Y-%m-%dT%H:%M:%S" "2023-02-12T12:24:30" == dtLocalTi
 def parseZonedTime? (fmt : String) (s : String) : Option ZonedTime :=
   parse TimeLocale.defaultTimeLocale fmt s
 
-def dtZonedTime : Option ZonedTime :=
-  some ⟨⟨fromGregorianDate dtDate, ⟨12, (by simp_arith)⟩, ⟨24, (by simp_arith)⟩,
-    TimeOfDay.toSecond 30 0 (by simp_arith) (by simp_arith)⟩, ⟨60,false,""⟩⟩
+def dtZonedTime : Option ZonedTime := some ⟨datetime% 2023-2-12 12:24:30, ⟨60,false,""⟩⟩
 
 example : parseZonedTime? "%Y-%m-%dT%H:%M:%S%Ez" "2023-02-12T12:24:30+01:00" == dtZonedTime := by
   native_decide
