Time/LocalTime/LocalTime.lean
@@ -1,4 +1,5 @@
 import Time.Calendar.Days
+import Time.Calendar.Gregorian
 import Time.Clock.DiffTime
 import Time.Clock.UTCTime
 import Time.LocalTime.TimeOfDay
@@ -11,11 +12,35 @@ structure LocalTime where
   localTimeOfDay : TimeOfDay
   deriving Repr, BEq
 
+namespace Time.Notation
+
+/-- LocalTime syntactic category -/
+declare_syntax_cat datetime
+/-- LocalTime from numeric literals year, month, day, hour, minute and second -/
+syntax num noWs "-" noWs num noWs "-" noWs num ws num noWs ":" noWs num (noWs ":" noWs num)? : datetime
+syntax "datetime%" datetime : term
+
+/--
+  `datetime% year-month-day hour:minute:second` is notation for
+  `(⟨Time.fromGregorianDate (Time.Date.mk year ⟨month, by omega⟩ ⟨day, by omega⟩ (by native_decide)),
+    Time.TimeOfDay.mk ⟨hour, by omega⟩ ⟨minute, by omega⟩ (Time.TimeOfDay.toSecond second 0 (by omega) (by omega))⟩
+    : Time.LocalTime)`
+  for the numeric literals year, month, day, hour, minute and second.
+-/
+macro_rules
+| `(datetime% $y:num-$mo:num-$d:num $h:num:$mi:num$[:$s:num]?) =>
+    `((⟨Time.fromGregorianDate (Time.Date.mk $y ⟨$mo, by omega⟩ ⟨$d, by omega⟩ (by native_decide)),
+      Time.TimeOfDay.mk ⟨$h, by omega⟩ ⟨$mi, by omega⟩
+        (Time.TimeOfDay.toSecond $(s.getD (Lean.Quote.quote 0)) 0 (by omega) (by omega))⟩
+      : Time.LocalTime))
+
+end Time.Notation
+
 instance : ToString LocalTime where
   toString a := s!"{a.localDay}, {a.localTimeOfDay}"
 
 instance : Inhabited LocalTime where
-  default := ⟨⟨0⟩, default⟩
+  default := ⟨default, default⟩
 
 namespace LocalTime
 
